Set post-condition for MlKemKeyPair::from in types.rs

libcrux-ml-kem/src/types.rs
@@ -140,6 +140,7 @@ pub struct MlKemKeyPair<const PRIVATE_KEY_SIZE: usize, const PUBLIC_KEY_SIZE: us
     pub(crate) pk: MlKemPublicKey<PUBLIC_KEY_SIZE>,
 }
 
+#[hax_lib::attributes]
 impl<const PRIVATE_KEY_SIZE: usize, const PUBLIC_KEY_SIZE: usize>
     MlKemKeyPair<PRIVATE_KEY_SIZE, PUBLIC_KEY_SIZE>
 {
@@ -152,6 +153,7 @@ impl<const PRIVATE_KEY_SIZE: usize, const PUBLIC_KEY_SIZE: usize>
     }
 
     /// Create a new [`MlKemKeyPair`] from the secret and public key.
+    #[ensures(|result| fstar!("${result}.f_sk == $sk /\\ ${result}.f_pk == $pk"))]
     pub fn from(
         sk: MlKemPrivateKey<PRIVATE_KEY_SIZE>,
         pk: MlKemPublicKey<PUBLIC_KEY_SIZE>,
