libcrux-ml-kem/proofs/fstar/extraction/Libcrux_ml_kem.Types.fsti
@@ -4,22 +4,22 @@ open Core
 open FStar.Mul
 
 /// The number of bytes
-val impl_6__len: v_SIZE: usize -> Prims.unit
+val impl_5__len: v_SIZE: usize -> Prims.unit
   -> Prims.Pure usize Prims.l_True (fun _ -> Prims.l_True)
 
 /// The number of bytes
-val impl_12__len: v_SIZE: usize -> Prims.unit
+val impl_11__len: v_SIZE: usize -> Prims.unit
   -> Prims.Pure usize Prims.l_True (fun _ -> Prims.l_True)
 
 /// The number of bytes
-val impl_18__len: v_SIZE: usize -> Prims.unit
+val impl_17__len: v_SIZE: usize -> Prims.unit
   -> Prims.Pure usize Prims.l_True (fun _ -> Prims.l_True)
 
 ///An ML-KEM Ciphertext
 type t_MlKemCiphertext (v_SIZE: usize) = { f_value:t_Array u8 v_SIZE }
 
 [@@ FStar.Tactics.Typeclasses.tcinstance]
-let impl_1 (v_SIZE: usize) : Core.Convert.t_AsRef (t_MlKemCiphertext v_SIZE) (t_Slice u8) =
+let impl (v_SIZE: usize) : Core.Convert.t_AsRef (t_MlKemCiphertext v_SIZE) (t_Slice u8) =
   {
     f_as_ref_pre = (fun (self: t_MlKemCiphertext v_SIZE) -> true);
     f_as_ref_post = (fun (self: t_MlKemCiphertext v_SIZE) (out: t_Slice u8) -> true);
@@ -27,7 +27,7 @@ let impl_1 (v_SIZE: usize) : Core.Convert.t_AsRef (t_MlKemCiphertext v_SIZE) (t_
   }
 
 [@@ FStar.Tactics.Typeclasses.tcinstance]
-let impl_2 (v_SIZE: usize) : Core.Convert.t_From (t_MlKemCiphertext v_SIZE) (t_Array u8 v_SIZE) =
+let impl_1 (v_SIZE: usize) : Core.Convert.t_From (t_MlKemCiphertext v_SIZE) (t_Array u8 v_SIZE) =
   {
     f_from_pre = (fun (value: t_Array u8 v_SIZE) -> true);
     f_from_post = (fun (value: t_Array u8 v_SIZE) (out: t_MlKemCiphertext v_SIZE) -> true);
@@ -35,7 +35,7 @@ let impl_2 (v_SIZE: usize) : Core.Convert.t_From (t_MlKemCiphertext v_SIZE) (t_A
   }
 
 [@@ FStar.Tactics.Typeclasses.tcinstance]
-let impl_3 (v_SIZE: usize) : Core.Convert.t_From (t_MlKemCiphertext v_SIZE) (t_Array u8 v_SIZE) =
+let impl_2 (v_SIZE: usize) : Core.Convert.t_From (t_MlKemCiphertext v_SIZE) (t_Array u8 v_SIZE) =
   {
     f_from_pre = (fun (value: t_Array u8 v_SIZE) -> true);
     f_from_post = (fun (value: t_Array u8 v_SIZE) (out: t_MlKemCiphertext v_SIZE) -> true);
@@ -48,7 +48,7 @@ let impl_3 (v_SIZE: usize) : Core.Convert.t_From (t_MlKemCiphertext v_SIZE) (t_A
   }
 
 [@@ FStar.Tactics.Typeclasses.tcinstance]
-let impl_4 (v_SIZE: usize) : Core.Convert.t_From (t_Array u8 v_SIZE) (t_MlKemCiphertext v_SIZE) =
+let impl_3 (v_SIZE: usize) : Core.Convert.t_From (t_Array u8 v_SIZE) (t_MlKemCiphertext v_SIZE) =
   {
     f_from_pre = (fun (value: t_MlKemCiphertext v_SIZE) -> true);
     f_from_post = (fun (value: t_MlKemCiphertext v_SIZE) (out: t_Array u8 v_SIZE) -> true);
@@ -56,14 +56,14 @@ let impl_4 (v_SIZE: usize) : Core.Convert.t_From (t_Array u8 v_SIZE) (t_MlKemCip
   }
 
 /// A reference to the raw byte slice.
-val impl_6__as_slice (v_SIZE: usize) (self: t_MlKemCiphertext v_SIZE)
+val impl_5__as_slice (v_SIZE: usize) (self: t_MlKemCiphertext v_SIZE)
     : Prims.Pure (t_Array u8 v_SIZE) Prims.l_True (fun _ -> Prims.l_True)
 
 ///An ML-KEM Private key
 type t_MlKemPrivateKey (v_SIZE: usize) = { f_value:t_Array u8 v_SIZE }
 
 [@@ FStar.Tactics.Typeclasses.tcinstance]
-let impl_7 (v_SIZE: usize) : Core.Convert.t_AsRef (t_MlKemPrivateKey v_SIZE) (t_Slice u8) =
+let impl_6 (v_SIZE: usize) : Core.Convert.t_AsRef (t_MlKemPrivateKey v_SIZE) (t_Slice u8) =
   {
     f_as_ref_pre = (fun (self: t_MlKemPrivateKey v_SIZE) -> true);
     f_as_ref_post = (fun (self: t_MlKemPrivateKey v_SIZE) (out: t_Slice u8) -> true);
@@ -71,7 +71,7 @@ let impl_7 (v_SIZE: usize) : Core.Convert.t_AsRef (t_MlKemPrivateKey v_SIZE) (t_
   }
 
 [@@ FStar.Tactics.Typeclasses.tcinstance]
-let impl_8 (v_SIZE: usize) : Core.Convert.t_From (t_MlKemPrivateKey v_SIZE) (t_Array u8 v_SIZE) =
+let impl_7 (v_SIZE: usize) : Core.Convert.t_From (t_MlKemPrivateKey v_SIZE) (t_Array u8 v_SIZE) =
   {
     f_from_pre = (fun (value: t_Array u8 v_SIZE) -> true);
     f_from_post = (fun (value: t_Array u8 v_SIZE) (out: t_MlKemPrivateKey v_SIZE) -> true);
@@ -79,7 +79,7 @@ let impl_8 (v_SIZE: usize) : Core.Convert.t_From (t_MlKemPrivateKey v_SIZE) (t_A
   }
 
 [@@ FStar.Tactics.Typeclasses.tcinstance]
-let impl_9 (v_SIZE: usize) : Core.Convert.t_From (t_MlKemPrivateKey v_SIZE) (t_Array u8 v_SIZE) =
+let impl_8 (v_SIZE: usize) : Core.Convert.t_From (t_MlKemPrivateKey v_SIZE) (t_Array u8 v_SIZE) =
   {
     f_from_pre = (fun (value: t_Array u8 v_SIZE) -> true);
     f_from_post = (fun (value: t_Array u8 v_SIZE) (out: t_MlKemPrivateKey v_SIZE) -> true);
@@ -92,7 +92,7 @@ let impl_9 (v_SIZE: usize) : Core.Convert.t_From (t_MlKemPrivateKey v_SIZE) (t_A
   }
 
 [@@ FStar.Tactics.Typeclasses.tcinstance]
-let impl_10 (v_SIZE: usize) : Core.Convert.t_From (t_Array u8 v_SIZE) (t_MlKemPrivateKey v_SIZE) =
+let impl_9 (v_SIZE: usize) : Core.Convert.t_From (t_Array u8 v_SIZE) (t_MlKemPrivateKey v_SIZE) =
   {
     f_from_pre = (fun (value: t_MlKemPrivateKey v_SIZE) -> true);
     f_from_post = (fun (value: t_MlKemPrivateKey v_SIZE) (out: t_Array u8 v_SIZE) -> true);
@@ -100,14 +100,14 @@ let impl_10 (v_SIZE: usize) : Core.Convert.t_From (t_Array u8 v_SIZE) (t_MlKemPr
   }
 
 /// A reference to the raw byte slice.
-val impl_12__as_slice (v_SIZE: usize) (self: t_MlKemPrivateKey v_SIZE)
+val impl_11__as_slice (v_SIZE: usize) (self: t_MlKemPrivateKey v_SIZE)
     : Prims.Pure (t_Array u8 v_SIZE) Prims.l_True (fun _ -> Prims.l_True)
 
 ///An ML-KEM Public key
 type t_MlKemPublicKey (v_SIZE: usize) = { f_value:t_Array u8 v_SIZE }
 
 [@@ FStar.Tactics.Typeclasses.tcinstance]
-let impl_13 (v_SIZE: usize) : Core.Convert.t_AsRef (t_MlKemPublicKey v_SIZE) (t_Slice u8) =
+let impl_12 (v_SIZE: usize) : Core.Convert.t_AsRef (t_MlKemPublicKey v_SIZE) (t_Slice u8) =
   {
     f_as_ref_pre = (fun (self: t_MlKemPublicKey v_SIZE) -> true);
     f_as_ref_post = (fun (self: t_MlKemPublicKey v_SIZE) (out: t_Slice u8) -> true);
@@ -115,7 +115,7 @@ let impl_13 (v_SIZE: usize) : Core.Convert.t_AsRef (t_MlKemPublicKey v_SIZE) (t_
   }
 
 [@@ FStar.Tactics.Typeclasses.tcinstance]
-let impl_14 (v_SIZE: usize) : Core.Convert.t_From (t_MlKemPublicKey v_SIZE) (t_Array u8 v_SIZE) =
+let impl_13 (v_SIZE: usize) : Core.Convert.t_From (t_MlKemPublicKey v_SIZE) (t_Array u8 v_SIZE) =
   {
     f_from_pre = (fun (value: t_Array u8 v_SIZE) -> true);
     f_from_post = (fun (value: t_Array u8 v_SIZE) (out: t_MlKemPublicKey v_SIZE) -> true);
@@ -123,7 +123,7 @@ let impl_14 (v_SIZE: usize) : Core.Convert.t_From (t_MlKemPublicKey v_SIZE) (t_A
   }
 
 [@@ FStar.Tactics.Typeclasses.tcinstance]
-let impl_15 (v_SIZE: usize) : Core.Convert.t_From (t_MlKemPublicKey v_SIZE) (t_Array u8 v_SIZE) =
+let impl_14 (v_SIZE: usize) : Core.Convert.t_From (t_MlKemPublicKey v_SIZE) (t_Array u8 v_SIZE) =
   {
     f_from_pre = (fun (value: t_Array u8 v_SIZE) -> true);
     f_from_post = (fun (value: t_Array u8 v_SIZE) (out: t_MlKemPublicKey v_SIZE) -> true);
@@ -136,7 +136,7 @@ let impl_15 (v_SIZE: usize) : Core.Convert.t_From (t_MlKemPublicKey v_SIZE) (t_A
   }
 
 [@@ FStar.Tactics.Typeclasses.tcinstance]
-let impl_16 (v_SIZE: usize) : Core.Convert.t_From (t_Array u8 v_SIZE) (t_MlKemPublicKey v_SIZE) =
+let impl_15 (v_SIZE: usize) : Core.Convert.t_From (t_Array u8 v_SIZE) (t_MlKemPublicKey v_SIZE) =
   {
     f_from_pre = (fun (value: t_MlKemPublicKey v_SIZE) -> true);
     f_from_post = (fun (value: t_MlKemPublicKey v_SIZE) (out: t_Array u8 v_SIZE) -> true);
@@ -144,11 +144,11 @@ let impl_16 (v_SIZE: usize) : Core.Convert.t_From (t_Array u8 v_SIZE) (t_MlKemPu
   }
 
 /// A reference to the raw byte slice.
-val impl_18__as_slice (v_SIZE: usize) (self: t_MlKemPublicKey v_SIZE)
+val impl_17__as_slice (v_SIZE: usize) (self: t_MlKemPublicKey v_SIZE)
     : Prims.Pure (t_Array u8 v_SIZE) Prims.l_True (fun _ -> Prims.l_True)
 
 [@@ FStar.Tactics.Typeclasses.tcinstance]
-let impl_5 (v_SIZE: usize) : Core.Convert.t_TryFrom (t_MlKemCiphertext v_SIZE) (t_Slice u8) =
+let impl_4 (v_SIZE: usize) : Core.Convert.t_TryFrom (t_MlKemCiphertext v_SIZE) (t_Slice u8) =
   {
     f_Error = Core.Array.t_TryFromSliceError;
     f_try_from_pre = (fun (value: t_Slice u8) -> true);
@@ -179,7 +179,7 @@ let impl_5 (v_SIZE: usize) : Core.Convert.t_TryFrom (t_MlKemCiphertext v_SIZE) (
   }
 
 [@@ FStar.Tactics.Typeclasses.tcinstance]
-let impl_11 (v_SIZE: usize) : Core.Convert.t_TryFrom (t_MlKemPrivateKey v_SIZE) (t_Slice u8) =
+let impl_10 (v_SIZE: usize) : Core.Convert.t_TryFrom (t_MlKemPrivateKey v_SIZE) (t_Slice u8) =
   {
     f_Error = Core.Array.t_TryFromSliceError;
     f_try_from_pre = (fun (value: t_Slice u8) -> true);
@@ -210,7 +210,7 @@ let impl_11 (v_SIZE: usize) : Core.Convert.t_TryFrom (t_MlKemPrivateKey v_SIZE) 
   }
 
 [@@ FStar.Tactics.Typeclasses.tcinstance]
-let impl_17 (v_SIZE: usize) : Core.Convert.t_TryFrom (t_MlKemPublicKey v_SIZE) (t_Slice u8) =
+let impl_16 (v_SIZE: usize) : Core.Convert.t_TryFrom (t_MlKemPublicKey v_SIZE) (t_Slice u8) =
   {
     f_Error = Core.Array.t_TryFromSliceError;
     f_try_from_pre = (fun (value: t_Slice u8) -> true);
@@ -247,16 +247,19 @@ type t_MlKemKeyPair (v_PRIVATE_KEY_SIZE: usize) (v_PUBLIC_KEY_SIZE: usize) = {
 }
 
 /// Create a new [`MlKemKeyPair`] from the secret and public key.
-val impl__from
+val impl_18__from
       (v_PRIVATE_KEY_SIZE v_PUBLIC_KEY_SIZE: usize)
       (sk: t_MlKemPrivateKey v_PRIVATE_KEY_SIZE)
       (pk: t_MlKemPublicKey v_PUBLIC_KEY_SIZE)
     : Prims.Pure (t_MlKemKeyPair v_PRIVATE_KEY_SIZE v_PUBLIC_KEY_SIZE)
       Prims.l_True
-      (fun _ -> Prims.l_True)
+      (ensures
+        fun result ->
+          let result:t_MlKemKeyPair v_PRIVATE_KEY_SIZE v_PUBLIC_KEY_SIZE = result in
+          result.f_sk == sk /\ result.f_pk == pk)
 
 /// Separate this key into the public and private key.
-val impl__into_parts
+val impl_18__into_parts
       (v_PRIVATE_KEY_SIZE v_PUBLIC_KEY_SIZE: usize)
       (self: t_MlKemKeyPair v_PRIVATE_KEY_SIZE v_PUBLIC_KEY_SIZE)
     : Prims.Pure (t_MlKemPrivateKey v_PRIVATE_KEY_SIZE & t_MlKemPublicKey v_PUBLIC_KEY_SIZE)
@@ -264,7 +267,7 @@ val impl__into_parts
       (fun _ -> Prims.l_True)
 
 /// Creates a new [`MlKemKeyPair`].
-val impl__new
+val impl_18__new
       (v_PRIVATE_KEY_SIZE v_PUBLIC_KEY_SIZE: usize)
       (sk: t_Array u8 v_PRIVATE_KEY_SIZE)
       (pk: t_Array u8 v_PUBLIC_KEY_SIZE)
@@ -273,25 +276,25 @@ val impl__new
       (fun _ -> Prims.l_True)
 
 /// Get a reference to the raw public key bytes.
-val impl__pk
+val impl_18__pk
       (v_PRIVATE_KEY_SIZE v_PUBLIC_KEY_SIZE: usize)
       (self: t_MlKemKeyPair v_PRIVATE_KEY_SIZE v_PUBLIC_KEY_SIZE)
     : Prims.Pure (t_Array u8 v_PUBLIC_KEY_SIZE) Prims.l_True (fun _ -> Prims.l_True)
 
 /// Get a reference to the [`MlKemPrivateKey<PRIVATE_KEY_SIZE>`].
-val impl__private_key
+val impl_18__private_key
       (v_PRIVATE_KEY_SIZE v_PUBLIC_KEY_SIZE: usize)
       (self: t_MlKemKeyPair v_PRIVATE_KEY_SIZE v_PUBLIC_KEY_SIZE)
     : Prims.Pure (t_MlKemPrivateKey v_PRIVATE_KEY_SIZE) Prims.l_True (fun _ -> Prims.l_True)
 
 /// Get a reference to the [`MlKemPublicKey<PUBLIC_KEY_SIZE>`].
-val impl__public_key
+val impl_18__public_key
       (v_PRIVATE_KEY_SIZE v_PUBLIC_KEY_SIZE: usize)
       (self: t_MlKemKeyPair v_PRIVATE_KEY_SIZE v_PUBLIC_KEY_SIZE)
     : Prims.Pure (t_MlKemPublicKey v_PUBLIC_KEY_SIZE) Prims.l_True (fun _ -> Prims.l_True)
 
 /// Get a reference to the raw private key bytes.
-val impl__sk
+val impl_18__sk
       (v_PRIVATE_KEY_SIZE v_PUBLIC_KEY_SIZE: usize)
       (self: t_MlKemKeyPair v_PRIVATE_KEY_SIZE v_PUBLIC_KEY_SIZE)
     : Prims.Pure (t_Array u8 v_PRIVATE_KEY_SIZE) Prims.l_True (fun _ -> Prims.l_True)
