libcrux-ml-kem/proofs/fstar/extraction/Libcrux_ml_kem.Ind_cca.fst
@@ -44,7 +44,6 @@ let serialize_kem_secret_key
         <:
         t_Slice u8)
   in
-  assert (Seq.slice out 0 (v (Spec.MLKEM.v_CPA_PRIVATE_KEY_SIZE v_K)) == private_key);
   let pointer:usize = pointer +! (Core.Slice.impl__len #u8 private_key <: usize) in
   let out:t_Array u8 v_SERIALIZED_KEY_LEN =
     Rust_primitives.Hax.Monomorphized_update_at.update_at_range out
@@ -69,10 +68,8 @@ let serialize_kem_secret_key
         <:
         t_Slice u8)
   in
-  assert (Seq.slice out 0 (v (Spec.MLKEM.v_CPA_PRIVATE_KEY_SIZE v_K)) == private_key);
-  assert (Seq.slice out (v (Spec.MLKEM.v_CPA_PRIVATE_KEY_SIZE v_K)) (v (Spec.MLKEM.v_CPA_PRIVATE_KEY_SIZE v_K) + v (Spec.MLKEM.v_CPA_PUBLIC_KEY_SIZE v_K)) == public_key);
   let pointer:usize = pointer +! (Core.Slice.impl__len #u8 public_key <: usize) in
-  let out1:t_Array u8 v_SERIALIZED_KEY_LEN =
+  let out:t_Array u8 v_SERIALIZED_KEY_LEN =
     Rust_primitives.Hax.Monomorphized_update_at.update_at_range out
       ({
           Core.Ops.Range.f_start = pointer;
@@ -126,8 +123,6 @@ let serialize_kem_secret_key
         <:
         t_Slice u8)
   in
-  admit();
-  Seq.lemma_eq_intro out (Seq.append (Seq.append (Seq.append private_key public_key) (Spec.Utils.v_H public_key)) implicit_rejection_value);
   out
 
 let validate_public_key
@@ -331,7 +326,7 @@ let encapsulate
           (Rust_primitives.unsize (Libcrux_ml_kem.Hash_functions.f_H #v_Hasher
                   #v_K
                   #FStar.Tactics.Typeclasses.solve
-                  (Rust_primitives.unsize (Libcrux_ml_kem.Types.impl_18__as_slice v_PUBLIC_KEY_SIZE
+                  (Rust_primitives.unsize (Libcrux_ml_kem.Types.impl_17__as_slice v_PUBLIC_KEY_SIZE
                           public_key
                         <:
                         t_Array u8 v_PUBLIC_KEY_SIZE)
@@ -359,7 +354,7 @@ let encapsulate
     Libcrux_ml_kem.Ind_cpa.encrypt v_K v_CIPHERTEXT_SIZE v_T_AS_NTT_ENCODED_SIZE v_C1_SIZE v_C2_SIZE
       v_VECTOR_U_COMPRESSION_FACTOR v_VECTOR_V_COMPRESSION_FACTOR v_C1_BLOCK_SIZE v_ETA1
       v_ETA1_RANDOMNESS_SIZE v_ETA2 v_ETA2_RANDOMNESS_SIZE #v_Vector #v_Hasher
-      (Rust_primitives.unsize (Libcrux_ml_kem.Types.impl_18__as_slice v_PUBLIC_KEY_SIZE public_key
+      (Rust_primitives.unsize (Libcrux_ml_kem.Types.impl_17__as_slice v_PUBLIC_KEY_SIZE public_key
             <:
             t_Array u8 v_PUBLIC_KEY_SIZE)
         <:
@@ -384,7 +379,6 @@ let encapsulate
   <:
   (Libcrux_ml_kem.Types.t_MlKemCiphertext v_CIPHERTEXT_SIZE & t_Array u8 (sz 32))
 
-#push-options "--z3rlimit 500"
 let generate_keypair
       (v_K v_CPA_PRIVATE_KEY_SIZE v_PRIVATE_KEY_SIZE v_PUBLIC_KEY_SIZE v_RANKED_BYTES_PER_RING_ELEMENT v_ETA1 v_ETA1_RANDOMNESS_SIZE:
           usize)
@@ -439,7 +433,7 @@ let generate_keypair
       #FStar.Tactics.Typeclasses.solve
       secret_key_serialized
   in
-  Libcrux_ml_kem.Types.impl__from v_PRIVATE_KEY_SIZE
+  Libcrux_ml_kem.Types.impl_18__from v_PRIVATE_KEY_SIZE
     v_PUBLIC_KEY_SIZE
     private_key
     (Core.Convert.f_from #(Libcrux_ml_kem.Types.t_MlKemPublicKey v_PUBLIC_KEY_SIZE)
